shorten long lines

UpdateDeprecations/Basic.lean
@@ -14,7 +14,8 @@ This file contains the code to perform the auto-replacements of `deprecated` dec
 Running `lake exe update_deprecations` assumes that there is a working cache and
 uses the information from deprecations to automatically substitute deprecated declarations.
 
-The script handles namespacing, replacing a possibly non-fully-qualified, deprecated name with the fully-qualified non-deprecated name.
+The script handles namespacing, replacing a possibly non-fully-qualified,
+deprecated name with the fully-qualified non-deprecated name.
 
 It also handles dot-notation.
 
@@ -41,42 +42,46 @@ def List.getCommon {α} [BEq α] : List α → List α → List α × List α ×
     else
       (common, l::left, r::right)
 
-/-- `splitWithNamespace fullName dotNot` returns `(common, declName, (termName, rightComponents))`, where
+/-- `splitWithNamespace fullName dotNot` returns `(common, declName, (termName, rightComponents))`,
+where
 * `fullName = declName ++ common`;
 * `dotNot = termName ++ common ++ rightComponents`
 
-and `common` is as large as possible, subject to the constraint that `rightComponents` does *not* contain
-a segment equal to the last segment of `fullName`.
+and `common` is as large as possible, subject to the constraint that `rightComponents` does *not*
+contain a segment equal to the last segment of `fullName`.
 
 For example, with input `Nat.Prime.ne_two` and `hp.ne_two.symm` it returns
 `(["ne_two"], ["Nat", "Prime"], (["hp"], ["symm"]))`.
 Assuming the restriction on the right-most occurrence mentioned above, we can therefore deduce that
 * the type of `hp` is `Nat.Prime`, i.e. `hp : Nat.Prime`;
 * the lemma `Nat.Prime.ne_two` exists;
-* the type of `hp.ne_two` is something that has a `.symm` in its namespace, i.e. `hp.ne_two : xx` and `xx.symm` exists
-  (in this case, `xx = Ne`).
+* the type of `hp.ne_two` is something that has a `.symm` in its namespace, i.e. `hp.ne_two : xx`
+  and `xx.symm` exists (in this case, `xx = Ne`).
 -/
-def splitWithNamespace (fullName dotNot : String) : List String × List String × (List String × List String) :=
+def splitWithNamespace (fullName dotNot : String) :
+    List String × List String × (List String × List String) :=
   let fns := (fullName.splitOn ".").reverse
   let dotns := (dotNot.splitOn ".").reverse
   let tail := fns.headD ""
-  --if tail == "" then none else
   let rightMostCommon := dotns.dropWhile (· != tail)  -- consider using matches further left as well
-  --if rightMostCommon == [] then none else
   let (common, fns', rm') := (List.getCommon fns) rightMostCommon
   (common.reverse, fns'.reverse, (rm'.reverse, (dotns.takeWhile (· != tail)).reverse))
 
-/-- `mIntercalate l` similar to `".".intercalate l`, except that it returns `[]` if the input list if `[]` and
+/-- `mIntercalate l` similar to `".".intercalate l`, except that
+it returns `[]` if the input list if `[]` and
 it returns the singleton list `[".".intercalate l]` otherwise. -/
 def mIntercalate (l : List String) : List String :=
   match ".".intercalate l with
     | "" => []
     | str => [str]
 
-/-- `recombineNamespace fullName dotNot newName` returns a candidate for "fixing" a deprecation in a namespace.
+/-- `recombineNamespace fullName dotNot newName` returns a candidate for "fixing" a deprecation in
+a namespace.
 * `dotNot` is a string representing dot-notation being used and involving a deprecated name
-* `fullName` is the fully-qualified string associated to the name that is deprecated and appears in `dotNot`
-* `newName` is the fully-qualified string associated to the name that is the non-deprecated version of `fullName`
+* `fullName` is the fully-qualified string associated to the name that is deprecated and appears
+  in `dotNot`
+* `newName` is the fully-qualified string associated to the name that is the non-deprecated version
+  of `fullName`
 
 It returns `none` if the final segment of `fullName` does not appear in `dotName`.
 -/
@@ -119,7 +124,8 @@ structure ReplData :=
 
 /-- `ReplData.newLine r` returns the new line obtained by performing the substitution,
 taking into account the deprecation.
-If no substitution is necessary, then it returns `none`: this is an indication that something went wrong. -/
+If no substitution is necessary, then it returns `none`: this is an indication that something went
+wrong. -/
 def ReplData.newLine (r : ReplData) (lines : Array String) : Option String :=
   let line := lines.getD (r.line - 1) ""
   match findFirstEnd r.fullName (line.drop r.col) with
@@ -129,32 +135,38 @@ def ReplData.newLine (r : ReplData) (lines : Array String) : Option String :=
         line.take r.col ++ t ++ line.drop (r.col + s.length)
       else none
 
-/-- We put the lexicographic order on the pairs `(line, col)` of `ReplData`, placing first positions that happen later.
+/-- We put the lexicographic order on the pairs `(line, col)` of `ReplData`,
+placing first positions that happen later.
 Most substitutions work on a line-by-line basis, so this is not necessary for "line information".
-However, in order to preserve column information, it is easier to perform the replacements on any given line from
-right to left.
-Since in the future some replacements may span several lines (or remove some of them), working backwards on the lines
-seems reasonable as well. -/
+However, in order to preserve column information, it is easier to perform the replacements
+on any given line from right to left.
+Since in the future some replacements may span several lines (or remove some of them),
+working backwards on the lines seems reasonable as well. -/
 instance : LT ReplData where
   lt a b := (b.line < a.line) || (a.line == b.line && b.col < a.col)
 
-theorem ReplData.lt_iff {a b : ReplData} : a < b ↔ (b.line < a.line) || (a.line == b.line && b.col < a.col) := by rfl
+theorem ReplData.lt_iff {a b : ReplData} :
+    a < b ↔ (b.line < a.line) || (a.line == b.line && b.col < a.col) := by
+  rfl
 
 instance : DecidableRel (LT.lt (α := ReplData)) := fun _ _ => decidable_of_iff' _ ReplData.lt_iff
 
-/-- `substitutions lines dat` takes as input the array `lines` of strings and the "instructions"
-`dat : Array ReplData`.
-The elements of `dat` contain the `(line, col)` information of the start of each `(deprecatedName, newName)` pair.
+/-- `substitutions lines dat` takes as input the array `lines` of strings and
+the "instructions" `dat : Array ReplData`.
+The elements of `dat` contain the `(line, col)` information of the start of each
+`(deprecatedName, newName)` pair.
 
-For each replacement instruction, if the substring of `lines[line]!` starting at `col` is "compatible" with being
-a `deprecatedName`, then `substitutions` replaces `deprecatedName` with a possible use of `newName`.
+For each replacement instruction, if the substring of `lines[line]!` starting at `col` is
+"compatible" with being a `deprecatedName`, then `substitutions` replaces `deprecatedName`
+with a possible use of `newName`.
 Otherwise, it leaves the string unchanged.
 
 Once all the instructions have been parsed, `substitutions` returns a count of the number of
 successful substitutions, the number of unsuccessful substitutions and the array of strings
 incorporating all the substitutions.
 -/
-def substitutions (lines : Array String) (dat : Array ReplData) : (Nat × Nat) × Array String := Id.run do
+def substitutions (lines : Array String) (dat : Array ReplData) : (Nat × Nat) × Array String :=
+  Id.run do
   let mut new := lines
   let mut replaced := 0
   let mut unreplaced := 0
@@ -182,7 +194,8 @@ def getBuild (mods : Array String := #[]) : IO String := do
   let build ← IO.Process.output { cmd := "lake", args := #["build", "--no-build"] ++ mods }
   if build.exitCode != 0 then
     IO.println s!"`lake build --no-build` failed: the oleans may be out of date oleans. \
-                Try running `lake build{mods.foldl (init := "") fun x y => s!"{x} {y}"}` or `lake exe cache get` first"
+                Try running `lake build{mods.foldl (init := "") fun x y => s!"{x} {y}"}` \
+                or `lake exe cache get` first"
     return default
   return build.stdout
 
@@ -230,10 +243,10 @@ def toFile : TSyntax `build → System.FilePath
 
 section elabs
 
-/-- `FromLinter` is the `HashMap` storing information about corrections that can be read off from the output of
-`lake build`.
-Each `System.FilePath` contains an array of `ReplData` containing information about `(deprecatedName, newName)` and
-the `(line, col)` pairs with the start of the deprecation.
+/-- `FromLinter` is the `HashMap` storing information about corrections that can be read off
+from the output of `lake build`.
+Each `System.FilePath` contains an array of `ReplData` containing information about
+`(deprecatedName, newName)` and the `(line, col)` pairs with the start of the deprecation.
 -/
 abbrev FromLinter := HashMap System.FilePath (Array ReplData)
 
@@ -268,7 +281,8 @@ elab bds:build* tk:"Build completed successfully." : command => do
     if noFiles == 0 then m!"No modifications needed"
     else if modifiedFiles.toArray.all (fun (_, _, x) => x == 0) then
       let totalModifications := modifiedFiles.fold (fun a _ (x, _) => a + x) 0
-      let toMo := m!"{totalModifications} modification" ++ if totalModifications == 1 then m!"" else "s"
+      let toMo := m!"{totalModifications} modification" ++
+        if totalModifications == 1 then m!"" else "s"
       let moFi := m!" across {noFiles} file" ++ if noFiles == 1 then m!"" else "s"
       toMo ++ moFi ++ ", all successful"
     else
@@ -315,7 +329,8 @@ def updateDeprecations : Cli.Cmd := `[Cli|
   You can run this on some modules only, using the optional `--mods`-flag: running\n\n\
   lake exe update_deprecations --mods One.Two.Three,Dd.Ee.Ff\n\n\
   only updates the deprecations in `One.Two.Three` and `Dd.Ee.Ff`. \
-  Note that you should provide a comma-separated list of module names, with no spaces between them. \
+  Note that you should provide a comma-separated list of module names, with no spaces between \
+  them. \
   As a convenience, the script tries to parse *paths* instead of *module names*: \
   passing\n\n\
   lake exe update_deprecations --mods One/Two/Three.lean,Dd.Ee.Ff\n\n\
